SafeAccess.v
@@ -1,0 +1,142 @@
+From Coq Require Import Arith.
+
+From Elo Require Import Map.
+From Elo Require Import Core.
+From Elo Require Import Access.
+
+Inductive SafeAccess (m : mem) : tm -> addr -> Prop :=
+  | safe_access_mem : forall ad ad' T,
+    ad <> ad' ->
+    SafeAccess m m[ad'] ad ->
+    SafeAccess m <{ &ad' :: T }> ad
+
+  | safe_access_ref : forall ad T,
+    SafeAccess m <{ &ad :: i&T }> ad
+
+  | safe_access_new : forall T t ad,
+    SafeAccess m t ad ->
+    SafeAccess m <{ new T t }> ad
+
+  | safe_access_load : forall t ad,
+    SafeAccess m t ad ->
+    SafeAccess m <{ *t }> ad
+
+  | safe_access_asg1 : forall t1 t2 ad,
+    SafeAccess m t1 ad ->
+    SafeAccess m <{ t1 = t2 }> ad
+
+  | safe_access_asg2 : forall t1 t2 ad,
+    SafeAccess m t2 ad ->
+    SafeAccess m <{ t1 = t2 }> ad
+
+  | safe_access_fun : forall x Tx t ad,
+    SafeAccess m t ad ->
+    SafeAccess m <{ fn x Tx --> t }> ad
+
+  | safe_access_call1 : forall t1 t2 ad,
+    SafeAccess m t1 ad ->
+    SafeAccess m <{ call t1 t2 }> ad
+
+  | safe_access_call2 : forall t1 t2 ad,
+    SafeAccess m t2 ad ->
+    SafeAccess m <{ call t1 t2 }> ad
+
+  | safe_access_seq1 : forall t1 t2 ad,
+    SafeAccess m t1 ad ->
+    SafeAccess m <{ t1; t2 }> ad
+
+  | safe_access_seq2 : forall t1 t2 ad,
+    SafeAccess m t2 ad ->
+    SafeAccess m <{ t1; t2 }> ad
+  .
+
+Inductive UnsafeAccess (m : mem) : tm -> addr -> Prop :=
+  | unsafe_access_mem : forall ad ad' T,
+    ad <> ad' ->
+    UnsafeAccess m m[ad'] ad ->
+    UnsafeAccess m <{ &ad' :: T }> ad
+
+  | unsafe_access_ref : forall ad T,
+    UnsafeAccess m <{ &ad :: &T }> ad
+
+  | unsafe_access_new : forall T t ad,
+    UnsafeAccess m t ad ->
+    UnsafeAccess m <{ new T t }> ad
+
+  | unsafe_access_load : forall t ad,
+    UnsafeAccess m t ad ->
+    UnsafeAccess m <{ *t }> ad
+
+  | unsafe_access_asg1 : forall t1 t2 ad,
+    UnsafeAccess m t1 ad ->
+    UnsafeAccess m <{ t1 = t2 }> ad
+
+  | unsafe_access_asg2 : forall t1 t2 ad,
+    UnsafeAccess m t2 ad ->
+    UnsafeAccess m <{ t1 = t2 }> ad
+
+  | unsafe_access_fun : forall x Tx t ad,
+    UnsafeAccess m t ad ->
+    UnsafeAccess m <{ fn x Tx --> t }> ad
+
+  | unsafe_access_call1 : forall t1 t2 ad,
+    UnsafeAccess m t1 ad ->
+    UnsafeAccess m <{ call t1 t2 }> ad
+
+  | unsafe_access_call2 : forall t1 t2 ad,
+    UnsafeAccess m t2 ad ->
+    UnsafeAccess m <{ call t1 t2 }> ad
+
+  | unsafe_access_seq1 : forall t1 t2 ad,
+    UnsafeAccess m t1 ad ->
+    UnsafeAccess m <{ t1; t2 }> ad
+
+  | unsafe_access_seq2 : forall t1 t2 ad,
+    UnsafeAccess m t2 ad ->
+    UnsafeAccess m <{ t1; t2 }> ad
+  .
+
+Theorem safe_access_then_access : forall m t ad,
+  SafeAccess m t ad ->
+  access m t ad.
+Proof.
+  intros * Hsacc. induction Hsacc; eauto using access.
+Qed.
+
+Theorem unsafe_access_then_access : forall m t ad,
+  UnsafeAccess m t ad ->
+  access m t ad.
+Proof.
+  intros * Huacc. induction Huacc; eauto using access.
+Qed.
+
+Theorem access_then_safe_or_unsafe_access : forall Gamma m t ad T,
+  Gamma |-- t is T ->
+  access m t ad ->
+  (SafeAccess m t ad \/ UnsafeAccess m t ad).
+Proof.
+  intros * Htype Hacc. generalize dependent Gamma. generalize dependent T.
+  induction Hacc; intros; inversion Htype; subst;
+  try (
+    match goal with
+    | H  : _ |-- ?t is _,
+      IH : forall _ _, _ |-- ?t is _ -> _ \/ _
+      |- _ =>
+      specialize (IH _ _ H) as [? | ?]
+    end
+  );
+  try solve
+    [ left; eauto using SafeAccess
+    | right; eauto using UnsafeAccess
+    ].
+  - right. destruct (Nat.eq_dec ad ad'); subst; eauto using UnsafeAccess.
+    eapply unsafe_access_mem; trivial.
+    admit.
+  - left.
+    admit.
+Qed.
+
+
+
+
+
