ValidAccesses.v
@@ -1,0 +1,282 @@
+From Coq Require Import Arith.Arith.
+From Coq Require Import Lia.
+
+From Elo Require Import Array.
+From Elo Require Import Core.
+From Elo Require Import Access.
+
+Definition valid_accesses (m : mem) (t : tm) :=
+  forall ad, access m t ad -> ad < length m.
+
+(* ------------------------------------------------------------------------- *)
+(* va constructors                                                           *)
+(* ------------------------------------------------------------------------- *)
+
+Local Ltac solve_constructor_va := 
+  intros; intros ? ?; inversion_access; eauto.
+
+Local Lemma va_new: forall m t T,
+  valid_accesses m t ->
+  valid_accesses m <{ new T t }>.
+Proof. solve_constructor_va. Qed.
+
+Local Lemma va_load : forall m t,
+  valid_accesses m t ->
+  valid_accesses m <{ *t }>.
+Proof. solve_constructor_va. Qed.
+
+Local Lemma va_asg : forall m t1 t2,
+  valid_accesses m t1 ->
+  valid_accesses m t2 ->
+  valid_accesses m <{ t1 = t2 }>.
+Proof. solve_constructor_va. Qed.
+
+Local Lemma va_fun : forall m x Tx t,
+  valid_accesses m t ->
+  valid_accesses m <{ fn x Tx --> t }>.
+Proof. solve_constructor_va. Qed.
+
+Local Lemma va_call : forall m t1 t2,
+  valid_accesses m t1 ->
+  valid_accesses m t2 ->
+  valid_accesses m <{ call t1 t2 }>.
+Proof. solve_constructor_va. Qed.
+
+Local Lemma va_seq : forall m t1 t2,
+  valid_accesses m t1 ->
+  valid_accesses m t2 ->
+  valid_accesses m <{ t1; t2 }>.
+Proof. solve_constructor_va. Qed.
+
+(* ------------------------------------------------------------------------- *)
+(* inversion-va                                                              *)
+(* ------------------------------------------------------------------------- *)
+
+Local Ltac solve_inversion_va := 
+  intros; unfold valid_accesses in *;
+  match goal with
+  | [ |- _ /\ _ ] => split
+  | [ |- _ ] => idtac
+  end;
+  eauto using access.
+
+Local Lemma inversion_va_ref : forall m ad T,
+  valid_accesses m <{ &ad :: T }> ->
+  valid_accesses m m[ad].
+Proof.
+  intros; unfold valid_accesses in *; eauto using access.
+  intros ad'. destruct (Nat.eq_dec ad ad'); subst; eauto using access.
+Qed.
+
+Local Lemma inversion_va_new : forall m t T,
+  valid_accesses m <{ new T t }> ->
+  valid_accesses m t.
+Proof. solve_inversion_va. Qed.
+
+Local Lemma inversion_va_load : forall m t,
+  valid_accesses m <{ *t }> ->
+  valid_accesses m t.
+Proof. solve_inversion_va. Qed.
+
+Local Lemma inversion_va_asg : forall m t1 t2,
+  valid_accesses m <{ t1 = t2 }> ->
+  valid_accesses m t1 /\ valid_accesses m t2.
+Proof. solve_inversion_va. Qed.
+
+Local Lemma inversion_va_fun : forall m x Tx t,
+  valid_accesses m <{ fn x Tx --> t }> ->
+  valid_accesses m t.
+Proof. solve_inversion_va. Qed.
+
+Local Lemma inversion_va_call : forall m t1 t2,
+  valid_accesses m <{ call t1 t2 }> ->
+  valid_accesses m t1 /\ valid_accesses m t2.
+Proof. solve_inversion_va. Qed.
+
+Local Lemma inversion_va_seq : forall m t1 t2,
+  valid_accesses m <{ t1; t2 }> ->
+  valid_accesses m t1 /\ valid_accesses m t2.
+Proof. solve_inversion_va. Qed.
+
+Ltac inversion_va :=
+  match goal with
+    | [ H : valid_accesses _ <{ &_ :: _ }>      |- _ ] =>
+        eapply inversion_va_ref in H as Hwba'
+    | [ H : valid_accesses _ <{ new _ _ }>      |- _ ] =>
+        eapply inversion_va_new in H
+    | [ H : valid_accesses _ <{ *_ }>           |- _ ] =>
+        eapply inversion_va_load in H
+    | [ H : valid_accesses _ <{ _ = _ }>        |- _ ] => 
+        eapply inversion_va_asg in H as [? ?]
+    | [ H : valid_accesses _ <{ fn _ _ --> _ }> |- _ ] => 
+        eapply inversion_va_fun in H
+    | [ H : valid_accesses _ <{ call _ _ }>     |- _ ] => 
+        eapply inversion_va_call in H as [? ?]
+    | [ H : valid_accesses _ <{ _; _ }>         |- _ ] => 
+        eapply inversion_va_seq in H as [? ?]
+  end.
+
+(* ------------------------------------------------------------------------- *)
+(* va -- value, mem & subst                                                  *)
+(* ------------------------------------------------------------------------- *)
+
+Local Lemma va_alloc_value : forall m t t' ad v,
+  valid_accesses m t ->
+  t --[EF_Alloc ad v]--> t' ->
+  valid_accesses m v.
+Proof.
+  intros. induction_step; inversion_va; eauto using access.
+Qed.
+
+Local Lemma va_write_value : forall m t t' ad v,
+  valid_accesses m t ->
+  t --[EF_Write ad v]--> t' ->
+  valid_accesses m v.
+Proof.
+  intros. induction_step; inversion_va; eauto using access.
+Qed.
+
+Local Lemma va_added_value : forall m v T,
+  valid_accesses (m +++ v) v ->
+  valid_accesses (m +++ v) <{ &(length m) :: T }>.
+Proof.
+  intros * ? ? Hacc.
+  remember (add m v) as m'.
+  remember (TM_Ref T (length m)) as t'.
+  induction Hacc; inversion Heqt'; subst.
+  - do 2 (rewrite_array TM_Unit). eauto using access.
+  - rewrite add_increments_length. lia.
+Qed.
+
+Local Lemma va_mem_add : forall m t v,
+  valid_accesses m t ->
+  valid_accesses (m +++ v) t.
+Proof.
+  intros * Hva ? Hacc. induction Hacc; subst; inversion_va; eauto.
+  - eapply IHHacc. intros ? ?.
+    destruct (lt_eq_lt_dec ad' (length m)) as [[? | ?] | ?]; subst;
+    do 3 (rewrite_array TM_Unit); eauto; try solve [inversion_access].
+    specialize (Hva (length m) (access_ref m (length m) _)). lia.
+  - rewrite add_increments_length. eauto using access, Nat.lt_lt_succ_r.
+Qed.
+
+Local Lemma va_mem_set : forall m t ad v,
+  valid_accesses m v ->
+  valid_accesses m t ->
+  valid_accesses m[ad <- v] t.
+Proof.
+  intros * ? ? ? Hacc.
+  rewrite set_preserves_length.
+  induction Hacc; inversion_va; eauto using access.
+  destruct (Nat.eq_dec ad ad'); subst;
+  assert (ad' < length m) by eauto using access;
+  do 2 (rewrite_array TM_Unit); eauto using access.
+Qed.
+
+Local Lemma va_subst : forall m t tx x,
+  valid_accesses m t ->
+  valid_accesses m tx ->
+  valid_accesses m ([x := tx] t).
+Proof.
+  intros. induction t;
+  try inversion_va; simpl; try (destruct String.string_dec);
+  eauto using va_new, va_load, va_asg, va_call, va_seq, va_fun.
+  intros ? F. inversion F.
+Qed.
+
+(* ------------------------------------------------------------------------- *)
+(* valid-accesses-preservation                                               *)
+(* ------------------------------------------------------------------------- *)
+
+Local Lemma va_none_preservation : forall m t t',
+  valid_accesses m t ->
+  t --[EF_None]--> t' ->
+  valid_accesses m t'.
+Proof.
+  intros. induction_step; inversion_va;
+  eauto using va_new, va_load, va_asg, va_fun, va_call, va_seq. 
+  inversion_va. eauto using va_subst.
+Qed.
+
+Local Lemma va_alloc_preservation : forall m t t' v,
+  valid_accesses m t ->
+  t --[EF_Alloc (length m) v]--> t' ->
+  valid_accesses (m +++ v) t'.
+Proof.
+  intros. induction_step; inversion_va;
+  eauto using va_new, va_load, va_asg, va_call, va_seq, va_mem_add,
+    va_added_value. 
+Qed.
+
+Local Lemma va_read_preservation : forall m t t' ad,
+  valid_accesses m t ->
+  t --[EF_Read ad m[ad]]--> t' ->
+  valid_accesses m t'.
+Proof.
+  intros. induction_step; inversion_va;
+  eauto using va_new, va_load, va_asg, va_call, va_seq.
+  intros ad' ?. destruct (Nat.eq_dec ad ad'); subst; eauto using access.
+Qed.
+
+Local Lemma va_write_preservation : forall m t t' ad v,
+  valid_accesses m t ->
+  t --[EF_Write ad v]--> t' ->
+  valid_accesses m[ad <- v] t'.
+Proof.
+  intros.
+  assert (valid_accesses m v); eauto using va_write_value.
+  induction_step; inversion_va;
+  eauto using va_new, va_load, va_asg, va_call, va_seq, va_mem_set.
+  intros ? ?. inversion_access.
+Qed.
+
+Theorem va_mstep_preservation : forall m m' t t' eff,
+  valid_accesses m t ->
+  m / t ==[eff]==> m' / t' ->
+  valid_accesses m' t'.
+Proof.
+  intros. inversion_mstep;
+  eauto using va_none_preservation,
+    va_alloc_preservation,
+    va_read_preservation,
+    va_write_preservation.
+Qed.
+
+(* ------------------------------------------------------------------------- *)
+(* memory valid-accesses preservation                                        *)
+(* ------------------------------------------------------------------------- *)
+
+Local Lemma mva_alloc_preservation : forall m t t' v,
+  valid_accesses m t ->
+  forall_memory m (valid_accesses m) ->
+  t --[EF_Alloc (length m) v]--> t' ->
+  forall_memory (m +++ v) (valid_accesses (m +++ v)).
+Proof.
+  intros * Hva ? ? ad. induction_step; inversion_va; eauto.
+  decompose sum (lt_eq_lt_dec ad (length m)); subst;
+  rewrite_array TM_Unit; eauto using va_mem_add.
+  intros ? ?. inversion_access.
+Qed.
+
+Local Lemma mva_write_preservation : forall m t t' ad v,
+  valid_accesses m t ->
+  forall_memory m (valid_accesses m) ->
+  t --[EF_Write ad v]--> t' ->
+  forall_memory m[ad <- v] (valid_accesses m[ad <- v]).
+Proof.
+  intros * Hva Hmva ? ad'. induction_step; inversion_va; eauto.
+  decompose sum (lt_eq_lt_dec ad ad'); subst;
+  try (assert (ad' < length m) by eauto using access);
+  rewrite_array TM_Unit; eauto using va_mem_set.
+Qed.
+
+Theorem mva_mstep_preservation : forall m m' t t' eff,
+  valid_accesses m t ->
+  forall_memory m (valid_accesses m) ->
+  m / t ==[eff]==> m' / t' ->
+  forall_memory m' (valid_accesses m').
+Proof.
+  intros. inversion_mstep;
+  eauto using mva_alloc_preservation, mva_write_preservation.
+Qed.
+
